Add do notation

Monad.v
@@ -1,6 +1,8 @@
+Require Import Utf8.
+
 Definition State {S : Type} (A : Type) := S -> (A * S)%type.
 
-Definition return_state {A S : Type} (x : A) : State A :=
+Definition return_state {S A : Type} (x : A) : State A :=
   fun (st : S) => (x, st).
 
 Definition bind_state {S A B : Type} (m : @State S A) (f : A -> @State S B) 
@@ -11,4 +13,21 @@ Definition get {S : Type} : State S := fun st => (st, st).
 
 Definition put {S : Type} (st' : S) : @State S unit := fun st => (tt, st').
  
+Class Monad (M : Type -> Type) : Type :=
+{
+  returnM : forall A, A -> M A;
+  bind : forall A B, M A  -> (A -> M B) -> M B;
+}.
 
+Instance state_monad {S : Type} : Monad (@State S) := 
+{
+  returnM := (@return_state S);
+  bind := (@bind_state S);
+}.
+
+
+Notation "x '<<' y ; z" := (bind_state y (fun x => z))
+  (at level 20, y at level 100, z at level 200, only parsing).
+
+Notation "x ;; z" := (bind_state x (fun _ => z))
+    (at level 100, z at level 200, only parsing, right associativity).
