AbstractInterpreter.v
@@ -11,16 +11,17 @@ Open Scope com_scope.
 Fixpoint abstract_eval_aexp (e : aexp) : State parity :=
   match e with 
   | ANum n => return_state (extract_par n)
-  | AVar x => 
-      bind_state get (fun st => return_state (st x))
+  | AVar x =>
+      st << get ;
+      return_state (st x)
   | APlus p1 p2 => 
-      bind_state (abstract_eval_aexp p1)
-        (fun n1 => bind_state (abstract_eval_aexp p2)
-          (fun n2 => return_state (parity_plus n1 n2)))
+      p1' << (abstract_eval_aexp p1) ;
+      p2' << (abstract_eval_aexp p2) ;
+      return_state (parity_plus p1' p2')
   | AMult p1 p2 =>
-      bind_state (abstract_eval_aexp p1)
-        (fun n1 => bind_state (abstract_eval_aexp p2)
-          (fun n2 => return_state (parity_mult n1 n2)))
+      p1' << (abstract_eval_aexp p1) ;
+      p2' << (abstract_eval_aexp p2) ;
+      return_state (parity_mult p1' p2')
   end.
 
 Fixpoint beval_abstract (b : bexp) : State abstr_bool :=
@@ -28,17 +29,17 @@ Fixpoint beval_abstract (b : bexp) : State abstr_bool :=
   | BFalse => return_state (ab_false)
   | BTrue => return_state (ab_true)
   | BEq e1 e2 => 
-      bind_state (abstract_eval_aexp e1)
-        (fun n1 => bind_state (abstract_eval_aexp e2)
-          (fun n2 => return_state (parity_eq n1 n2)))
+      e1' << (abstract_eval_aexp e1) ;
+      e2' << (abstract_eval_aexp e2) ;
+      return_state (parity_eq e1' e2')
   | BLe e1 e2=> return_state ab_top
   | BNot b => 
-      bind_state (beval_abstract b)
-        (fun b => return_state (neg_ab b))
-  | BAnd b1 b2 => 
-      bind_state (beval_abstract b1)
-        (fun b1' => bind_state (beval_abstract b2)
-          (fun b2' => return_state (and_ab b1' b2')))
+      b' << (beval_abstract b) ;
+      return_state (neg_ab b')
+  | BAnd b1 b2 =>
+      b1' << (beval_abstract b1) ;
+      b2' << (beval_abstract b2) ;
+      return_state (and_ab b1' b2')
   end.
 
 Definition eval_if_abstract (b : abstr_bool) (st1 st2 : abstract_store) : abstract_store :=
@@ -52,13 +53,12 @@ Definition eval_if_abstract (b : abstr_bool) (st1 st2 : abstract_store) : abstra
 Fixpoint ceval_abstract (c : com) : State unit :=
   match c with
   | CSkip => return_state tt
-  | c1 ;; c2 =>
-      bind_state (ceval_abstract c1)
-        (fun _ => ceval_abstract c2)
+  | c1 ;c; c2 =>
+      (ceval_abstract c1) ;; (ceval_abstract c2)
   | x ::= a => 
-      bind_state (abstract_eval_aexp a)
-        (fun n => bind_state get 
-          (fun st => put (t_update st x n)))
+      p << (abstract_eval_aexp a) ;
+      st << get ;
+      put (t_update st x p)
   end.
 
 
