ConcreteInterpreter.v
@@ -1,4 +1,5 @@
 Require Import Coq.Arith.Arith.
+Require Import Utf8.
 
 Require Import Language.
 Require Import Maps.
@@ -11,15 +12,17 @@ Open Scope com_scope.
 Fixpoint eval_aexp (e : aexp) : State nat := 
   match e with
   | ANum n => return_state n
-  | AVar x => bind_state get (fun st => return_state (st x))
+  | AVar x => 
+      st << get ;
+      return_state (st x)
   | APlus e1 e2 => 
-      bind_state (eval_aexp e1) 
-        (fun n1 => bind_state (eval_aexp e2) 
-          (fun n2 => return_state (n1 + n2)))
+      n1 << (eval_aexp e1) ;
+      n2 << (eval_aexp e2) ;
+      return_state (n1 + n2)
   | AMult e1 e2 => 
-      bind_state (eval_aexp e2)
-        (fun n1 => bind_state (eval_aexp e2)
-          (fun n2 => return_state (n1 * n2)))
+      n1 << (eval_aexp e1) ;
+      n2 << (eval_aexp e2) ;
+      return_state (n1 + n2)
   end.
 
 Fixpoint eval_bexp (e : bexp) : State bool :=
@@ -27,19 +30,20 @@ Fixpoint eval_bexp (e : bexp) : State bool :=
   | BTrue => return_state true
   | BFalse => return_state false
   | BEq a1 a2 =>
-      bind_state (eval_aexp a1)
-        (fun n1 => bind_state (eval_aexp a2)
-          (fun n2 => return_state (Nat.eqb n1 n2)))
+      n1 << (eval_aexp a1) ;
+      n2 << (eval_aexp a2) ;
+      return_state (Nat.eqb n1 n2)
   | BLe a1 a2 =>
-      bind_state (eval_aexp a2)
-        (fun n1 => bind_state (eval_aexp a2)
-          (fun n2 => return_state (Nat.leb n1 n2)))
+      n1 << (eval_aexp a1) ;
+      n2 << (eval_aexp a2) ;
+      return_state (Nat.leb n1 n2)
   | BNot b => 
-      bind_state (eval_bexp b) (fun b => return_state (negb b))
+      b' << (eval_bexp b) ;
+      return_state (negb b')
   | BAnd b1 b2 =>
-      bind_state (eval_bexp b1) 
-        (fun b1 => bind_state (eval_bexp b2)
-          (fun b2 => return_state (andb b1 b2)))
+      b1' << (eval_bexp b1) ;
+      b2' << (eval_bexp b2) ;
+      return_state (andb b1' b2')
   end.
 
 Definition eval_if (b : bool) (st1 st2 : state) : state :=
@@ -48,8 +52,10 @@ Definition eval_if (b : bool) (st1 st2 : state) : state :=
 Fixpoint ceval (c : com) : State unit :=
   match c with
   | CSkip => return_state tt
-  | c1 ;; c2 => 
-      bind_state (ceval c1) (fun _ => ceval c2)
-  | x ::= a => bind_state (eval_aexp a) (fun (n : nat) => 
-      bind_state get (fun st => put (t_update st x n)))
+  | c1 ;c; c2 => 
+      (ceval c1) ;; (ceval c2)
+  | x ::= a => 
+      n << (eval_aexp a) ;
+      st << get ;
+      put (t_update st x n)
   end.
